Update goose output
Changed how structs are emitted, so significant changes throughout.

src/go_lang/examples/logging2.v
@@ -32,12 +32,6 @@ Module Log.
     "memTxnNxt" :: refT uint64T;
     "logTxnNxt" :: refT uint64T
   ].
-  Definition T: ty := struct.t S.
-  Definition Ptr: ty := struct.ptrT S.
-  Section fields.
-    Context `{ext_ty: ext_types}.
-    Definition get := struct.get S.
-  End fields.
 End Log.
 
 Definition Log__writeHdr: val :=
@@ -45,7 +39,7 @@ Definition Log__writeHdr: val :=
     let: "hdr" := NewSlice byteT #4096 in
     UInt64Put "hdr" "len";;
     disk.Write LOGCOMMIT "hdr".
-Theorem Log__writeHdr_t: ⊢ Log__writeHdr : (Log.T -> uint64T -> unitT).
+Theorem Log__writeHdr_t: ⊢ Log__writeHdr : (struct.t Log.S -> uint64T -> unitT).
 Proof. typecheck. Qed.
 Hint Resolve Log__writeHdr_t : types.
 
@@ -62,7 +56,7 @@ Definition Init: val :=
     ] in
     Log__writeHdr "log" #0;;
     "log".
-Theorem Init_t: ⊢ Init : (uint64T -> Log.T).
+Theorem Init_t: ⊢ Init : (uint64T -> struct.t Log.S).
 Proof. typecheck. Qed.
 Hint Resolve Init_t : types.
 
@@ -71,7 +65,7 @@ Definition Log__readHdr: val :=
     let: "hdr" := disk.Read LOGCOMMIT in
     let: "disklen" := UInt64Get "hdr" in
     "disklen".
-Theorem Log__readHdr_t: ⊢ Log__readHdr : (Log.T -> uint64T).
+Theorem Log__readHdr_t: ⊢ Log__readHdr : (struct.t Log.S -> uint64T).
 Proof. typecheck. Qed.
 Hint Resolve Log__readHdr_t : types.
 
@@ -84,18 +78,18 @@ Definition Log__readBlocks: val :=
       "blks" <- SliceAppend !"blks" "blk";;
       Continue);;
     !"blks".
-Theorem Log__readBlocks_t: ⊢ Log__readBlocks : (Log.T -> uint64T -> slice.T disk.blockT).
+Theorem Log__readBlocks_t: ⊢ Log__readBlocks : (struct.t Log.S -> uint64T -> slice.T disk.blockT).
 Proof. typecheck. Qed.
 Hint Resolve Log__readBlocks_t : types.
 
 Definition Log__Read: val :=
   λ: "log",
-    lock.acquire (Log.get "logLock" "log");;
+    lock.acquire (struct.get Log.S "logLock" "log");;
     let: "disklen" := Log__readHdr "log" in
     let: "blks" := Log__readBlocks "log" "disklen" in
-    lock.release (Log.get "logLock" "log");;
+    lock.release (struct.get Log.S "logLock" "log");;
     "blks".
-Theorem Log__Read_t: ⊢ Log__Read : (Log.T -> slice.T disk.blockT).
+Theorem Log__Read_t: ⊢ Log__Read : (struct.t Log.S -> slice.T disk.blockT).
 Proof. typecheck. Qed.
 Hint Resolve Log__Read_t : types.
 
@@ -104,38 +98,38 @@ Definition Log__memWrite: val :=
     let: "n" := slice.len "l" in
     let: "i" := ref #0 in
     (for: (!"i" < "n"); ("i" <- !"i" + #1) :=
-      Log.get "memLog" "log" <- SliceAppend (!(Log.get "memLog" "log")) (SliceGet "l" !"i");;
+      struct.get Log.S "memLog" "log" <- SliceAppend (!(struct.get Log.S "memLog" "log")) (SliceGet "l" !"i");;
       Continue).
-Theorem Log__memWrite_t: ⊢ Log__memWrite : (Log.T -> slice.T disk.blockT -> unitT).
+Theorem Log__memWrite_t: ⊢ Log__memWrite : (struct.t Log.S -> slice.T disk.blockT -> unitT).
 Proof. typecheck. Qed.
 Hint Resolve Log__memWrite_t : types.
 
 Definition Log__memAppend: val :=
   λ: "log" "l",
-    lock.acquire (Log.get "memLock" "log");;
-    (if: !(Log.get "memLen" "log") + slice.len "l" ≥ Log.get "logSz" "log"
+    lock.acquire (struct.get Log.S "memLock" "log");;
+    (if: !(struct.get Log.S "memLen" "log") + slice.len "l" ≥ struct.get Log.S "logSz" "log"
     then
-      lock.release (Log.get "memLock" "log");;
+      lock.release (struct.get Log.S "memLock" "log");;
       (#false, #0)
     else
-      let: "txn" := !(Log.get "memTxnNxt" "log") in
-      let: "n" := !(Log.get "memLen" "log") + slice.len "l" in
-      Log.get "memLen" "log" <- "n";;
-      Log.get "memTxnNxt" "log" <- !(Log.get "memTxnNxt" "log") + #1;;
-      lock.release (Log.get "memLock" "log");;
+      let: "txn" := !(struct.get Log.S "memTxnNxt" "log") in
+      let: "n" := !(struct.get Log.S "memLen" "log") + slice.len "l" in
+      struct.get Log.S "memLen" "log" <- "n";;
+      struct.get Log.S "memTxnNxt" "log" <- !(struct.get Log.S "memTxnNxt" "log") + #1;;
+      lock.release (struct.get Log.S "memLock" "log");;
       (#true, "txn")).
-Theorem Log__memAppend_t: ⊢ Log__memAppend : (Log.T -> slice.T disk.blockT -> (boolT * uint64T)).
+Theorem Log__memAppend_t: ⊢ Log__memAppend : (struct.t Log.S -> slice.T disk.blockT -> (boolT * uint64T)).
 Proof. typecheck. Qed.
 Hint Resolve Log__memAppend_t : types.
 
 (* XXX just an atomic read? *)
 Definition Log__readLogTxnNxt: val :=
   λ: "log",
-    lock.acquire (Log.get "memLock" "log");;
-    let: "n" := !(Log.get "logTxnNxt" "log") in
-    lock.release (Log.get "memLock" "log");;
+    lock.acquire (struct.get Log.S "memLock" "log");;
+    let: "n" := !(struct.get Log.S "logTxnNxt" "log") in
+    lock.release (struct.get Log.S "memLock" "log");;
     "n".
-Theorem Log__readLogTxnNxt_t: ⊢ Log__readLogTxnNxt : (Log.T -> uint64T).
+Theorem Log__readLogTxnNxt_t: ⊢ Log__readLogTxnNxt : (struct.t Log.S -> uint64T).
 Proof. typecheck. Qed.
 Hint Resolve Log__readLogTxnNxt_t : types.
 
@@ -147,7 +141,7 @@ Definition Log__diskAppendWait: val :=
       (if: "txn" < "logtxn"
       then Break
       else Continue)).
-Theorem Log__diskAppendWait_t: ⊢ Log__diskAppendWait : (Log.T -> uint64T -> unitT).
+Theorem Log__diskAppendWait_t: ⊢ Log__diskAppendWait : (struct.t Log.S -> uint64T -> unitT).
 Proof. typecheck. Qed.
 Hint Resolve Log__diskAppendWait_t : types.
 
@@ -160,7 +154,7 @@ Definition Log__Append: val :=
       #()
     else #());;
     "ok".
-Theorem Log__Append_t: ⊢ Log__Append : (Log.T -> slice.T disk.blockT -> boolT).
+Theorem Log__Append_t: ⊢ Log__Append : (struct.t Log.S -> slice.T disk.blockT -> boolT).
 Proof. typecheck. Qed.
 Hint Resolve Log__Append_t : types.
 
@@ -172,25 +166,25 @@ Definition Log__writeBlocks: val :=
       let: "bk" := SliceGet "l" !"i" in
       disk.Write ("pos" + !"i") "bk";;
       Continue).
-Theorem Log__writeBlocks_t: ⊢ Log__writeBlocks : (Log.T -> slice.T disk.blockT -> uint64T -> unitT).
+Theorem Log__writeBlocks_t: ⊢ Log__writeBlocks : (struct.t Log.S -> slice.T disk.blockT -> uint64T -> unitT).
 Proof. typecheck. Qed.
 Hint Resolve Log__writeBlocks_t : types.
 
 Definition Log__diskAppend: val :=
   λ: "log",
-    lock.acquire (Log.get "logLock" "log");;
+    lock.acquire (struct.get Log.S "logLock" "log");;
     let: "disklen" := Log__readHdr "log" in
-    lock.acquire (Log.get "memLock" "log");;
-    let: "memlen" := !(Log.get "memLen" "log") in
-    let: "allblks" := !(Log.get "memLog" "log") in
+    lock.acquire (struct.get Log.S "memLock" "log");;
+    let: "memlen" := !(struct.get Log.S "memLen" "log") in
+    let: "allblks" := !(struct.get Log.S "memLog" "log") in
     let: "blks" := SliceSkip "allblks" "disklen" in
-    let: "memnxt" := !(Log.get "memTxnNxt" "log") in
-    lock.release (Log.get "memLock" "log");;
+    let: "memnxt" := !(struct.get Log.S "memTxnNxt" "log") in
+    lock.release (struct.get Log.S "memLock" "log");;
     Log__writeBlocks "log" "blks" "disklen";;
     Log__writeHdr "log" "memlen";;
-    Log.get "logTxnNxt" "log" <- "memnxt";;
-    lock.release (Log.get "logLock" "log").
-Theorem Log__diskAppend_t: ⊢ Log__diskAppend : (Log.T -> unitT).
+    struct.get Log.S "logTxnNxt" "log" <- "memnxt";;
+    lock.release (struct.get Log.S "logLock" "log").
+Theorem Log__diskAppend_t: ⊢ Log__diskAppend : (struct.t Log.S -> unitT).
 Proof. typecheck. Qed.
 Hint Resolve Log__diskAppend_t : types.
 
@@ -200,7 +194,7 @@ Definition Log__Logger: val :=
     (for: (#true); (Skip) :=
       Log__diskAppend "log";;
       Continue).
-Theorem Log__Logger_t: ⊢ Log__Logger : (Log.T -> unitT).
+Theorem Log__Logger_t: ⊢ Log__Logger : (struct.t Log.S -> unitT).
 Proof. typecheck. Qed.
 Hint Resolve Log__Logger_t : types.
 
@@ -211,12 +205,6 @@ Module Txn.
     "log" :: struct.ptrT Log.S;
     "blks" :: mapT disk.blockT
   ].
-  Definition T: ty := struct.t S.
-  Definition Ptr: ty := struct.ptrT S.
-  Section fields.
-    Context `{ext_ty: ext_types}.
-    Definition get := struct.get S.
-  End fields.
 End Txn.
 
 (* XXX wait if cannot reserve space in log *)
@@ -227,48 +215,48 @@ Definition Begin: val :=
       "blks" ::= NewMap disk.blockT
     ] in
     "txn".
-Theorem Begin_t: ⊢ Begin : (struct.ptrT Log.S -> Txn.T).
+Theorem Begin_t: ⊢ Begin : (struct.ptrT Log.S -> struct.t Txn.S).
 Proof. typecheck. Qed.
 Hint Resolve Begin_t : types.
 
 Definition Txn__Write: val :=
   λ: "txn" "addr" "blk",
     let: "ret" := ref #true in
-    let: (<>, "ok") := MapGet (Txn.get "blks" "txn") "addr" in
+    let: (<>, "ok") := MapGet (struct.get Txn.S "blks" "txn") "addr" in
     (if: "ok"
     then
-      MapInsert (Txn.get "blks" "txn") "addr" !"blk";;
+      MapInsert (struct.get Txn.S "blks" "txn") "addr" !"blk";;
       #()
     else #());;
     (if: ~ "ok"
     then
-      (if: "addr" = LOGMAXBLK
+      (if: ("addr" = LOGMAXBLK)
       then "ret" <- #false
-      else MapInsert (Txn.get "blks" "txn") "addr" !"blk");;
+      else MapInsert (struct.get Txn.S "blks" "txn") "addr" !"blk");;
       #()
     else #());;
     !"ret".
-Theorem Txn__Write_t: ⊢ Txn__Write : (Txn.T -> uint64T -> refT disk.blockT -> boolT).
+Theorem Txn__Write_t: ⊢ Txn__Write : (struct.t Txn.S -> uint64T -> refT disk.blockT -> boolT).
 Proof. typecheck. Qed.
 Hint Resolve Txn__Write_t : types.
 
 Definition Txn__Read: val :=
   λ: "txn" "addr",
-    let: ("v", "ok") := MapGet (Txn.get "blks" "txn") "addr" in
+    let: ("v", "ok") := MapGet (struct.get Txn.S "blks" "txn") "addr" in
     (if: "ok"
     then "v"
     else disk.Read ("addr" + LOGEND)).
-Theorem Txn__Read_t: ⊢ Txn__Read : (Txn.T -> uint64T -> disk.blockT).
+Theorem Txn__Read_t: ⊢ Txn__Read : (struct.t Txn.S -> uint64T -> disk.blockT).
 Proof. typecheck. Qed.
 Hint Resolve Txn__Read_t : types.
 
 Definition Txn__Commit: val :=
   λ: "txn",
     let: "blks" := ref (zero_val (slice.T disk.blockT)) in
-    MapIter (Txn.get "blks" "txn") (λ: <> "v",
+    MapIter (struct.get Txn.S "blks" "txn") (λ: <> "v",
       "blks" <- SliceAppend !"blks" "v");;
-    let: "ok" := Log__Append (struct.load Log.S (Txn.get "log" "txn")) !"blks" in
+    let: "ok" := Log__Append (struct.load Log.S (struct.get Txn.S "log" "txn")) !"blks" in
     "ok".
-Theorem Txn__Commit_t: ⊢ Txn__Commit : (Txn.T -> boolT).
+Theorem Txn__Commit_t: ⊢ Txn__Commit : (struct.t Txn.S -> boolT).
 Proof. typecheck. Qed.
 Hint Resolve Txn__Commit_t : types.
