src/go_lang/examples/simpledb.v
@@ -70,7 +70,7 @@ Definition DecodeUInt64: val :=
 Definition DecodeEntry: val :=
   λ: "data",
     let: ("key", "l1") := DecodeUInt64 "data" in
-    (if: "l1" = #0
+    (if: ("l1" = #0)
     then
       (struct.mk Entry.S [
          "Key" ::= #0;
@@ -78,7 +78,7 @@ Definition DecodeEntry: val :=
        ], #0)
     else
       let: ("valueLen", "l2") := DecodeUInt64 (SliceSkip "data" "l1") in
-      (if: "l2" = #0
+      (if: ("l2" = #0)
       then
         (struct.mk Entry.S [
            "Key" ::= #0;
@@ -130,7 +130,7 @@ Definition readTableIndex: val :=
         Continue
       else
         let: "p" := FS.readAt "f" (lazyFileBuf.get "offset" !"buf" + slice.len (lazyFileBuf.get "next" !"buf")) #4096 in
-        (if: slice.len "p" = #0
+        (if: (slice.len "p" = #0)
         then Break
         else
           let: "newBuf" := SliceAppendSlice (lazyFileBuf.get "next" !"buf") "p" in
@@ -203,7 +203,7 @@ Definition newBuf: val :=
 Definition bufFlush: val :=
   λ: "f",
     let: "buf" := !(bufFile.get "buf" "f") in
-    (if: slice.len "buf" = #0
+    (if: (slice.len "buf" = #0)
     then #()
     else
       FS.append (bufFile.get "file" "f") "buf";;
@@ -382,10 +382,10 @@ Definition Write: val :=
 
 Definition freshTable: val :=
   λ: "p",
-    (if: "p" = #(str"table.0")
+    (if: ("p" = #(str"table.0"))
     then #(str"table.1")
     else
-      (if: "p" = #(str"table.1")
+      (if: ("p" = #(str"table.1"))
       then #(str"table.0")
       else "p")).
 
@@ -419,7 +419,7 @@ Definition tablePutOldTable: val :=
         Continue
       else
         let: "p" := FS.readAt (Table.get "File" "t") (lazyFileBuf.get "offset" !"buf" + slice.len (lazyFileBuf.get "next" !"buf")) #4096 in
-        (if: slice.len "p" = #0
+        (if: (slice.len "p" = #0)
         then Break
         else
           let: "newBuf" := SliceAppendSlice (lazyFileBuf.get "next" !"buf") "p" in
@@ -484,10 +484,10 @@ Definition recoverManifest: val :=
 (* delete 'name' if it isn't tableName or "manifest" *)
 Definition deleteOtherFile: val :=
   λ: "name" "tableName",
-    (if: "name" = "tableName"
+    (if: ("name" = "tableName")
     then #()
     else
-      (if: "name" = #(str"manifest")
+      (if: ("name" = #(str"manifest"))
       then #()
       else FS.delete #(str"db") "name")).
 
@@ -497,7 +497,7 @@ Definition deleteOtherFiles: val :=
     let: "nfiles" := slice.len "files" in
     let: "i" := ref #0 in
     (for: (#true); (Skip) :=
-      (if: !"i" = "nfiles"
+      (if: (!"i" = "nfiles")
       then Break
       else
         let: "name" := SliceGet "files" !"i" in
